e2e/WitnessRejectD.v
@@ -36,23 +36,23 @@ Definition o_short_two_origins : Compilable.outsides (prog [ Syntax.ShortVarDecl
 Definition r_short_dup_use : Compilable.rejects (prog [ Syntax.ShortVarDecl (Collections.MakeNonEmpty (Syntax.BNamed (OID "x")) [Syntax.BNamed (OID "x")]) (Collections.MakeNonEmpty (ILIT 1) [ILIT 2]) ; PL [ VNAME "x" ] ]). Proof. reject. Qed.
 
 Lemma reader_disp : Compilable.disposition rprobe = Compilable.Rejected.
-Proof. vm_compute; reflexivity. Qed.
+Proof. obs_disp. Qed.
 
-Lemma reader_disp_compiled : Compilable.disposition cprobe = Compilable.Compiled. Proof. vm_compute; reflexivity. Qed.
+Lemma reader_disp_compiled : Compilable.disposition cprobe = Compilable.Compiled. Proof. obs_disp. Qed.
 
-Lemma reader_index_compiled : AN.res_index (rres cprobe) = AN.res_index (AN.analyze cprobe). Proof. vm_compute; reflexivity. Qed.
+Lemma reader_index_compiled : AN.res_index (rres cprobe) = AN.res_index (AN.analyze cprobe). Proof. obs_eq cprobe. Qed.
 
-Lemma reader_index_outside : AN.res_index (rres oprobe) = AN.res_index (AN.analyze oprobe). Proof. vm_compute; reflexivity. Qed.
+Lemma reader_index_outside : AN.res_index (rres oprobe) = AN.res_index (AN.analyze oprobe). Proof. obs_eq oprobe. Qed.
 
 (* payload catalogue via the bp-free Report views: goal types carry no BindingPhase, so vm_compute stays cheap *)
 Definition r_iota_cause :
   RP.result_cause_views (rres (prog [ PL [ Syntax.Name (Names.predeclared_ordinary Names.PIota) ] ])) = [ RP.CvInvalidIdentity Names.PIota ].
-Proof. vm_compute; reflexivity. Qed.
+Proof. obs_direct (prog [ PL [ Syntax.Name (Names.predeclared_ordinary Names.PIota) ] ]). Qed.
 
 Definition o_cx_typed_payload :
   RP.result_cause_views (rres (prog [ PL [ CPLX (CONV Names.PFloat32 (ILIT 1)) (CONV Names.PFloat32 (ILIT 2)) ] ])) = []
   /\ RP.result_req_views (rres (prog [ PL [ CPLX (CONV Names.PFloat32 (ILIT 1)) (CONV Names.PFloat32 (ILIT 2)) ] ])) = [ RP.RvComplexType ].
-Proof. split; vm_compute; reflexivity. Qed.
+Proof. split; obs_direct (prog [ PL [ CPLX (CONV Names.PFloat32 (ILIT 1)) (CONV Names.PFloat32 (ILIT 2)) ] ]). Qed.
 
 Definition r_main_as_type : Compilable.rejects (prog [ Syntax.DeclarationStmt (Syntax.VarDecl [ Syntax.MakeVarSpec (NE1 (Syntax.BNamed (OID "x"))) (Syntax.VarTypeOnly (Syntax.NamedType (OID "main"))) ]) ]). Proof. reject. Qed.
 
@@ -65,25 +65,38 @@ Definition r_redecl_payload :
    | [ d ] => match RP.diag_group_name d with Some nm => Names.ordinary_equalb nm (OID "x") | None => false end
    | _ => false
    end) = true.
-Proof. vm_compute; reflexivity. Qed.
+Proof.
+  assert (H : map RP.diag_group_name (dsites (prog [ Syntax.DeclarationStmt (Syntax.VarDecl [ Syntax.MakeVarSpec (NE1 (Syntax.BNamed (OID "x"))) (Syntax.VarValues None (NE1 (ILIT 1))) ]) ; Syntax.DeclarationStmt (Syntax.VarDecl [ Syntax.MakeVarSpec (NE1 (Syntax.BNamed (OID "x"))) (Syntax.VarValues None (NE1 (ILIT 2))) ]) ])) = [ Some (OID "x") ]).
+  { unfold dsites.
+    assert (Hc : AN.collision_rows (rres (prog [ Syntax.DeclarationStmt (Syntax.VarDecl [ Syntax.MakeVarSpec (NE1 (Syntax.BNamed (OID "x"))) (Syntax.VarValues None (NE1 (ILIT 1))) ]) ; Syntax.DeclarationStmt (Syntax.VarDecl [ Syntax.MakeVarSpec (NE1 (Syntax.BNamed (OID "x"))) (Syntax.VarValues None (NE1 (ILIT 2))) ]) ])) = []) by (apply (proj1 (AN.dnc_iff _)); obs_seal (prog [ Syntax.DeclarationStmt (Syntax.VarDecl [ Syntax.MakeVarSpec (NE1 (Syntax.BNamed (OID "x"))) (Syntax.VarValues None (NE1 (ILIT 1))) ]) ; Syntax.DeclarationStmt (Syntax.VarDecl [ Syntax.MakeVarSpec (NE1 (Syntax.BNamed (OID "x"))) (Syntax.VarValues None (NE1 (ILIT 2))) ]) ])).
+    assert (Hm : AN.main_rows (rres (prog [ Syntax.DeclarationStmt (Syntax.VarDecl [ Syntax.MakeVarSpec (NE1 (Syntax.BNamed (OID "x"))) (Syntax.VarValues None (NE1 (ILIT 1))) ]) ; Syntax.DeclarationStmt (Syntax.VarDecl [ Syntax.MakeVarSpec (NE1 (Syntax.BNamed (OID "x"))) (Syntax.VarValues None (NE1 (ILIT 2))) ]) ])) = []) by (apply (proj1 (AN.dnm_iff _)); obs_seal (prog [ Syntax.DeclarationStmt (Syntax.VarDecl [ Syntax.MakeVarSpec (NE1 (Syntax.BNamed (OID "x"))) (Syntax.VarValues None (NE1 (ILIT 1))) ]) ; Syntax.DeclarationStmt (Syntax.VarDecl [ Syntax.MakeVarSpec (NE1 (Syntax.BNamed (OID "x"))) (Syntax.VarValues None (NE1 (ILIT 2))) ]) ])).
+    assert (Ho : AN.occ_diags (rres (prog [ Syntax.DeclarationStmt (Syntax.VarDecl [ Syntax.MakeVarSpec (NE1 (Syntax.BNamed (OID "x"))) (Syntax.VarValues None (NE1 (ILIT 1))) ]) ; Syntax.DeclarationStmt (Syntax.VarDecl [ Syntax.MakeVarSpec (NE1 (Syntax.BNamed (OID "x"))) (Syntax.VarValues None (NE1 (ILIT 2))) ]) ])) = []) by (apply (proj1 (AN.dncause_iff _)); obs_seal (prog [ Syntax.DeclarationStmt (Syntax.VarDecl [ Syntax.MakeVarSpec (NE1 (Syntax.BNamed (OID "x"))) (Syntax.VarValues None (NE1 (ILIT 1))) ]) ; Syntax.DeclarationStmt (Syntax.VarDecl [ Syntax.MakeVarSpec (NE1 (Syntax.BNamed (OID "x"))) (Syntax.VarValues None (NE1 (ILIT 2))) ]) ])).
+    rewrite (AN.diagnostics_order (rres (prog [ Syntax.DeclarationStmt (Syntax.VarDecl [ Syntax.MakeVarSpec (NE1 (Syntax.BNamed (OID "x"))) (Syntax.VarValues None (NE1 (ILIT 1))) ]) ; Syntax.DeclarationStmt (Syntax.VarDecl [ Syntax.MakeVarSpec (NE1 (Syntax.BNamed (OID "x"))) (Syntax.VarValues None (NE1 (ILIT 2))) ]) ]))), Hc, Hm, Ho. rewrite ?app_nil_l, ?app_nil_r.
+    unfold AN.group_rows; rewrite map_map.
+    erewrite (map_ext _ (fun rr => Some (projT1 rr))) by (intro rr; reflexivity).
+    unfold rres, result_of_compile, AN.res_binds, AN.res_bind_data, AN.res_surface, AN.res_index.
+    rewrite (Compilable.compile_observe_data (prog [ Syntax.DeclarationStmt (Syntax.VarDecl [ Syntax.MakeVarSpec (NE1 (Syntax.BNamed (OID "x"))) (Syntax.VarValues None (NE1 (ILIT 1))) ]) ; Syntax.DeclarationStmt (Syntax.VarDecl [ Syntax.MakeVarSpec (NE1 (Syntax.BNamed (OID "x"))) (Syntax.VarValues None (NE1 (ILIT 2))) ]) ])). vm_compute. reflexivity. }
+  destruct (dsites (prog [ Syntax.DeclarationStmt (Syntax.VarDecl [ Syntax.MakeVarSpec (NE1 (Syntax.BNamed (OID "x"))) (Syntax.VarValues None (NE1 (ILIT 1))) ]) ; Syntax.DeclarationStmt (Syntax.VarDecl [ Syntax.MakeVarSpec (NE1 (Syntax.BNamed (OID "x"))) (Syntax.VarValues None (NE1 (ILIT 2))) ]) ])) as [|d0 [|d1 r1]]; cbn in H; try discriminate H.
+  injection H as Hd0. cbn. rewrite Hd0. reflexivity.
+Qed.
 
 (* an unbound application head is a dependent non-result, never a successful application fact *)
 Definition r_unbound_app_dep :
   existsb (fun f => match f with AN.OFApp _ (AN.ADependent (AN.DepUnboundNameA _ _ _)) => true | _ => false end)
           (pfacts (prog [ Syntax.ExprStmt (APP (OID "undefined") []) ])) = true.
-Proof. vm_compute; reflexivity. Qed.
+Proof. obs_direct (prog [ Syntax.ExprStmt (APP (OID "undefined") []) ]). Qed.
 
 (* an expr-statement whose expr owns an issue is a dependent non-result, never a successful statement *)
 Definition r_child_stmt_dep :
   existsb (fun f => match f with AN.OFStmt _ (AN.SDependent _) => true | _ => false end)
           (pfacts (prog [ Syntax.ExprStmt (APP (Names.predeclared_ordinary Names.PIota) []) ])) = true.
-Proof. vm_compute; reflexivity. Qed.
+Proof. obs_direct (prog [ Syntax.ExprStmt (APP (Names.predeclared_ordinary Names.PIota) []) ]). Qed.
 
 (* a redeclared name used as a type is a dependent non-result, never a fabricated Bool type *)
 Definition r_redecl_type_dep :
   existsb (fun f => match f with AN.OFType _ (AN.TDependent _) => true | _ => false end)
           (pfacts (prog [ Syntax.DeclarationStmt (Syntax.VarDecl [ Syntax.MakeVarSpec (NE1 (Syntax.BNamed (OID "y"))) (Syntax.VarValues None (NE1 (ILIT 1))) ]) ; Syntax.DeclarationStmt (Syntax.VarDecl [ Syntax.MakeVarSpec (NE1 (Syntax.BNamed (OID "y"))) (Syntax.VarValues None (NE1 (ILIT 2))) ]) ; Syntax.DeclarationStmt (Syntax.VarDecl [ Syntax.MakeVarSpec (NE1 (Syntax.BNamed (OID "z"))) (Syntax.VarTypeOnly (Syntax.NamedType (OID "y"))) ]) ])) = true.
-Proof. vm_compute; reflexivity. Qed.
+Proof. obs_direct (prog [ Syntax.DeclarationStmt (Syntax.VarDecl [ Syntax.MakeVarSpec (NE1 (Syntax.BNamed (OID "y"))) (Syntax.VarValues None (NE1 (ILIT 1))) ]) ; Syntax.DeclarationStmt (Syntax.VarDecl [ Syntax.MakeVarSpec (NE1 (Syntax.BNamed (OID "y"))) (Syntax.VarValues None (NE1 (ILIT 2))) ]) ; Syntax.DeclarationStmt (Syntax.VarDecl [ Syntax.MakeVarSpec (NE1 (Syntax.BNamed (OID "z"))) (Syntax.VarTypeOnly (Syntax.NamedType (OID "y"))) ]) ]). Qed.
 
 (* (a) one fixed main, no competitor -> unique group + MainOne -> Compiled *)
 Definition c_main_only : Compilable.compiles (prog_tops [ main0 ]). Proof. compileok. Qed.
@@ -95,25 +108,85 @@ Definition r_main_multiple_payload :
   (match dsites (prog_tops [ main0 ; main0 ]) with
    | [ d ] => match RP.diag_group_name d with Some nm => Names.ordinary_equalb nm (OID "main") | None => false end
    | _ => false end) = true.
-Proof. vm_compute; reflexivity. Qed.
+Proof.
+  assert (H : map RP.diag_group_name (dsites (prog_tops [ main0 ; main0 ])) = [ Some (OID "main") ]).
+  { unfold dsites.
+    assert (Hc : AN.collision_rows (rres (prog_tops [ main0 ; main0 ])) = []) by (apply (proj1 (AN.dnc_iff _)); obs_seal (prog_tops [ main0 ; main0 ])).
+    assert (Hm : AN.main_rows (rres (prog_tops [ main0 ; main0 ])) = []) by (apply (proj1 (AN.dnm_iff _)); obs_seal (prog_tops [ main0 ; main0 ])).
+    assert (Ho : AN.occ_diags (rres (prog_tops [ main0 ; main0 ])) = []) by (apply (proj1 (AN.dncause_iff _)); obs_seal (prog_tops [ main0 ; main0 ])).
+    rewrite (AN.diagnostics_order (rres (prog_tops [ main0 ; main0 ]))), Hc, Hm, Ho. rewrite ?app_nil_l, ?app_nil_r.
+    unfold AN.group_rows; rewrite map_map.
+    erewrite (map_ext _ (fun rr => Some (projT1 rr))) by (intro rr; reflexivity).
+    unfold rres, result_of_compile, AN.res_binds, AN.res_bind_data, AN.res_surface, AN.res_index.
+    rewrite (Compilable.compile_observe_data (prog_tops [ main0 ; main0 ])). vm_compute. reflexivity. }
+  destruct (dsites (prog_tops [ main0 ; main0 ])) as [|d0 [|d1 r1]]; cbn in H; try discriminate H.
+  injection H as Hd0. cbn. rewrite Hd0. reflexivity.
+Qed.
 
 (* the output collision and a redeclared group coexist as distinct diagnostics through the one authority *)
 Definition d4_collision_redeclared_coexist :
   andb (existsb (fun d => match d with AN.DOutputCollision _ => true | _ => false end) (dsites p_collision_redecl))
        (existsb (fun d => match d with AN.DRedeclaredGroup _ => true | _ => false end) (dsites p_collision_redecl)) = true.
-Proof. vm_compute; reflexivity. Qed.
+Proof.
+  apply andb_true_intro. split.
+  - destruct (AN.result_collision_ref (rres p_collision_redecl)) as [cr|] eqn:Hcr.
+    2:{ exfalso. apply AN.collision_ref_none in Hcr. revert Hcr.
+        unfold rres, result_of_compile, AN.result_preflight, AN.res_pkg, AN.res_binds, AN.res_bind_data, AN.res_surface, AN.res_index.
+        rewrite (Compilable.compile_observe_data p_collision_redecl). vm_compute. discriminate. }
+    apply existsb_exists. exists (AN.DOutputCollision cr). split; [ | reflexivity ].
+    unfold dsites. rewrite (AN.diagnostics_order (rres p_collision_redecl)).
+    apply in_or_app. left. unfold AN.collision_rows. rewrite Hcr. left. reflexivity.
+  - assert (Hgr : AN.group_rows (rres p_collision_redecl) <> []).
+    { intro Hnil. apply (proj2 (AN.dnr_iff _)) in Hnil. revert Hnil.
+      unfold rres, result_of_compile, AN.data_no_redecl, AN.res_binds, AN.res_bind_data, AN.res_surface, AN.res_index.
+      rewrite (Compilable.compile_observe_data p_collision_redecl). vm_compute. discriminate. }
+    destruct (AN.group_rows (rres p_collision_redecl)) as [|g0 grest] eqn:Hg; [ exfalso; exact (Hgr eq_refl) | ].
+    apply existsb_exists. exists g0. split.
+    + unfold dsites. rewrite (AN.diagnostics_order (rres p_collision_redecl)).
+      apply in_or_app. right. apply in_or_app. right. apply in_or_app. left. rewrite Hg. left. reflexivity.
+    + revert Hg. unfold AN.group_rows.
+      destruct (AN.BN.redeclaration_roots (AN.res_binds (rres p_collision_redecl))) as [|r0 rr]; [ discriminate | ].
+      intro Hg. injection Hg as Hg0 _. subst g0. reflexivity.
+Qed.
 
 (* §17.2 a package with exactly one valid main has no missing-main case: the false missing-main cannot arise *)
 Lemma mm17_2_main_one_none : pmissing (prog_tops [ main0 ]) = [].
-Proof. vm_compute; reflexivity. Qed.
+Proof.
+  unfold pmissing, ppkg.
+  assert (Hnil : AN.result_missing_main_refs (rres (prog_tops [ main0 ])) = []).
+  { apply (map_eq_nil AN.mmr_package). rewrite AN.missing_main_packages.
+    unfold rres, result_of_compile, AN.is_missing, AN.result_package_rule, AN.res_binds, AN.res_surface, AN.res_bind_data, AN.res_index.
+    rewrite (Compilable.compile_observe_data (prog_tops [ main0 ])). vm_compute. reflexivity. }
+  rewrite Hnil. reflexivity.
+Qed.
 
 (* §17.3 a package with multiple mains is a group redeclaration, not a missing main: still no missing-main case *)
 Lemma mm17_3_main_multiple_none : pmissing (prog_tops [ main0 ; main0 ]) = [].
-Proof. vm_compute; reflexivity. Qed.
+Proof.
+  unfold pmissing, ppkg.
+  assert (Hnil : AN.result_missing_main_refs (rres (prog_tops [ main0 ; main0 ])) = []).
+  { apply (map_eq_nil AN.mmr_package). rewrite AN.missing_main_packages.
+    unfold rres, result_of_compile, AN.is_missing, AN.result_package_rule, AN.res_binds, AN.res_surface, AN.res_bind_data, AN.res_index.
+    rewrite (Compilable.compile_observe_data (prog_tops [ main0 ; main0 ])). vm_compute. reflexivity. }
+  rewrite Hnil. reflexivity.
+Qed.
 
 (* §17.4 an exact output collision retains the exact package+root: the collision view names the colliding entry *)
 Lemma mm17_4_collision_view : option_map RP.cv_root (pcollision p_collision) = Some "generated"%string.
-Proof. vm_compute; reflexivity. Qed.
+Proof.
+  unfold pcollision, ppkg.
+  destruct (AN.result_collision_ref (rres p_collision)) as [cr|] eqn:Hcr.
+  - cbn [option_map]. f_equal.
+    destruct (RP.collision_view_exact cr) as [_ Hcvr]. rewrite Hcvr.
+    transitivity (match AN.result_preflight (rres p_collision) with
+                  | AN.FreshCollision _ rr => PI.re_name rr | AN.FreshOk => ""%string end).
+    + rewrite (AN.collision_case _ cr); reflexivity.
+    + unfold rres, result_of_compile, AN.result_preflight, AN.res_pkg, AN.res_binds, AN.res_bind_data, AN.res_surface, AN.res_index;
+      rewrite (Compilable.compile_observe_data p_collision); vm_compute; reflexivity.
+  - exfalso. apply AN.collision_ref_none in Hcr. revert Hcr.
+    unfold rres, result_of_compile, AN.result_preflight, AN.res_pkg, AN.res_binds, AN.res_bind_data, AN.res_surface, AN.res_index;
+    rewrite (Compilable.compile_observe_data p_collision); vm_compute; discriminate.
+Qed.
 
 Definition dr_default_ovf : Compilable.rejects dp_default_ovf. Proof. reject. Qed.
 
